\section*{Aufgabe 1}
\subsection*{a)}
\paragraph*{$ V(c\cdot X)=c^2\cdot V(X) $:}
\begin{align*}
V(c\cdot X)&=\sum_{\omega\in\Omega}^{}((c\cdot X)(\omega)-E(c\cdot X))^2\cdot m(\omega)\\
&=\sum_{\omega\in\Omega}^{}(c\cdot X(\omega)-c\cdot E(X))^2\cdot m(\omega)\\
&=\sum_{\omega\in\Omega}^{}(c\cdot (X(\omega)-E(X)))^2\cdot m(\omega)\\
&=\sum_{\omega\in\Omega}^{}c^2\cdot (X(\omega)-E(X))^2\cdot m(\omega)\\
&=c^2\cdot\sum_{\omega\in\Omega}^{}(X(\omega)-E(X))^2\cdot m(\omega)\\
&=c^2\cdot V(X)
\end{align*}
\paragraph*{$ V(X+c)=V(X) $:}
\begin{align*}
V(X+c)&=\sum_{\omega\in\Omega}^{}((X+c)(\omega)-E(X+c))^2\cdot m(\omega)\\
&=\sum_{\omega\in\Omega}^{}(X(\omega)+\cancel{c}-E(X)-\cancel{c})^2\cdot m(\omega)\\
&=\sum_{\omega\in\Omega}^{}(X(\omega)-E(X))^2\cdot m(\omega)\\
&=V(X)
\end{align*}
\subsection*{b)}
\paragraph*{$ V(X_1\cdot X_2)=V(X_1)\cdot E(X_2)^2 + E(X_1)^2\cdot V(X_2) + V(X_1)\cdot V(X_2) $:}
/
