\pagebreak
\section*{Aufgabe 3}
Zu Beweisen: $ \alpha \rightarrow \beta\gamma \land \beta \rightarrow \delta \implies \alpha \rightarrow  \beta\delta\gamma $
\begin{enumerate}
\item $ \alpha \rightarrow \beta\gamma \land \beta \rightarrow \delta \implies \alpha \rightarrow  \beta\delta\gamma $ \quad (Gegeben)
\item $ \alpha \rightarrow \beta\gamma $ \quad (Vereinfachung aus 1.)
\item $ \beta \rightarrow \delta $ \quad (Vereinfachung aus 1.)
\item $ \alpha \rightarrow \beta $ \quad (Dekomposition aus 2.)
\item $ \alpha \rightarrow \delta $ \quad (Transitivit√§t aus 3. und 4.)
\item $ \alpha \rightarrow \beta\delta\gamma $ \quad (Vereinigungsregel aus 2. und 5.)
\end{enumerate}